\begin{align}
    \textbf{E}[\textbf{X}]=\int_{\Omega}{d\textbf{X}f(\textbf{X})}
\end{align}

\begin{align}
    S^{(1)}={\frac{1}{M}}{\sum_\textbf{X}{\frac{f(\textbf{X})}{p(\textbf{X})}}}
\end{align}

I vá»›i M $\rightarrow \infty$

\int_{\Omega}{d\textbf{X}p(\textbf{X})}=1

\begin{align}
    \int_{\Omega}{d\textbf{X}p(\textbf{X})}=1
\end{align}

\begin{align}
    \sigma^2=\left\{\int_{\Omega}d\textbf{X}\frac{f^2(\textbf{X})}{p(\textbf{X})}-\left[\int_{\Omega}d\textbf{X}f(\textbf{X})\right]^2\right\}M^{-1}
\end{align}

\sigma^2=\left\{\int_{\Omega}d\textbf{X}\frac{f^2(\textbf{X})}{p(\textbf{X})}-\left[\int_{\Omega}d\textbf{X}f(\textbf{X})\right]^2\right\}M^{-1}


\begin{align}
    S^{(1)}={\frac{1}{M}}{\sum_\textbf{X}{\frac{f(\textbf{X})}{p(\textbf{X})}}}
\end{align}

\begin{align}
    \sigma^2\cong\frac{S^{(2)}-S^{(1)}}{M-1}
\end{align}


\begin{align}
    S^{(2)}=\frac{1}{M}{\sum_\textbf{X}}\left(\frac{f(\textbf{X})}{p(\textbf{X})}\right)^2
\end{align}

